Move towards using [unchanged_at_extended]. See msg.
The issue with the previous approach is because we need to be
conservative. This in particular means that if we have both
[unchanged_at locs s1 s2] and [unchanged_except locs s1 s2], we **DO
NOT** have [unchanged_except Nil s1 s2], even thought it might seem
like we should.

An example that demonstrates this is if we assume that XMM1 is not
disjoint from RAX. This is a conservative assumption and is correct
and sound. However, at this point, we face our conundrum. Assume the
[locs] above is the singleton set [RAX]. Since [unchanged_at]
looks **only** at the locations within the [locs] and
[unchanged_except] looks at locations which are _strictly_ disjoint
from the [locs], the [XMM1] is not talked about whatsoever. This means
that with this definition, we have a situation where the [XMM1]
register _could_ have different values, and thus this is a
counter-example.

We fix this by extending [unchanged_at], to get
[unchanged_at_extended]. This new extended definition takes into
account everything that is not provably disjoint. This means that it
is more difficult to prove, but it provides much more if it were to
exist in the precondition. Additionally, it properly encodes the
notion of conservatively equal. Thus, with this definition, we can
now (trivially) show that [unchanged_at_extended locs s1 s2] and
[unchanged_except locs s1 s2] implies [unchanged_except Nil s1 s2].

It does throw some extra stuff into the picture; in particular, we can
no longer as easily show the behavior upon two operations that are
commuted. We need to introduce a new notion of
[unchanged_upon_both_non_disjoint] which allows one to talk about two
different sets of access locations; and is true only if their
intersection is maintained across both states.

It remains to be seen how much extra effort this new approach will
take up for proving things from [untainted_eval_ins] though.

vale/code/lib/transformers/Vale.Transformers.InstructionReorder.fst
@@ -1000,12 +1000,26 @@ let rec unchanged_at (locs:list access_location) (s1 s2:machine_state) : GTot Ty
       (unchanged_at xs s1 s2)
     )
 
+let rec unchanged_at_extended (locs:list access_location) (s1 s2:machine_state) : GTot Type0 =
+  (forall a. {:pattern (eval_access_location a s1) \/ (eval_access_location a s2)} (
+      (not !!(disjoint_access_location_from_locations a locs)) ==> (
+        (eval_access_location a s1 == eval_access_location a s2))))
+
+let rec lemma_unchanged_at_extended_implies_unchanged_at locs s1 s2 :
+  Lemma
+    (requires (unchanged_at_extended locs s1 s2))
+    (ensures (unchanged_at locs s1 s2)) =
+  match locs with
+  | [] -> ()
+  | x :: xs ->
+    lemma_unchanged_at_extended_implies_unchanged_at xs s1 s2
+
 let bounded_effects (reads writes:list access_location) (f:st unit) : GTot Type0 =
   (only_affects writes f) /\
   (
-    forall s1 s2. {:pattern unchanged_at writes (run f s1) (run f s2)} (
+    forall s1 s2. {:pattern unchanged_at_extended writes (run f s1) (run f s2)} (
       unchanged_at reads s1 s2 ==>
-      (unchanged_at writes (run f s1) (run f s2) /\
+      (unchanged_at_extended writes (run f s1) (run f s2) /\
        (run f s1).ms_ok = (run f s2).ms_ok)
     )
   )
@@ -1072,7 +1086,7 @@ let rec lemma_disjoint_access_location_from_locations_mem
 let rec lemma_unchanged_at_mem (as:list access_location) (a:access_location) (s1 s2:machine_state) :
   Lemma
     (requires (
-        (unchanged_at as s1 s2) /\
+        (unchanged_at_extended as s1 s2) /\
         (L.mem a as)))
     (ensures (
         (eval_access_location a s1 == eval_access_location a s2))) =
@@ -1082,65 +1096,35 @@ let rec lemma_unchanged_at_mem (as:list access_location) (a:access_location) (s1
     if a = x then () else
     lemma_unchanged_at_mem xs a s1 s2
 
+let unchanged_upon_both_non_disjoint (a1 a2:list access_location) (s1 s2:machine_state) =
+  (forall a. {:pattern (eval_access_location a s1) \/ (eval_access_location a s2)}
+     (
+       (not (!!(disjoint_access_location_from_locations a a1))) /\
+       (not (!!(disjoint_access_location_from_locations a a2)))
+     ) ==> (
+     eval_access_location a s1 == eval_access_location a s2
+   )
+  )
+
+
 let lemma_unchanged_at_combine (a1 a2:list access_location) (sa1 sa2 sb1 sb2:machine_state) :
   Lemma
     (requires (
         !!(disjoint_access_locations a1 a2 "") /\
-        (unchanged_at a1 sa1 sb2) /\
+        (unchanged_upon_both_non_disjoint a1 a2 sa1 sa2) /\
+        (unchanged_at_extended a1 sa1 sb2) /\
         (unchanged_except a2 sa1 sb1) /\
-        (unchanged_at a2 sa2 sb1) /\
+        (unchanged_at_extended a2 sa2 sb1) /\
         (unchanged_except a1 sa2 sb2)))
     (ensures (
-        (unchanged_at (a1 `L.append` a2) sb1 sb2))) =
-  let precond = !!(disjoint_access_locations a1 a2 "") /\
-                 (unchanged_at a1 sa1 sb2) /\
-                 (unchanged_except a2 sa1 sb1) /\
-                 (unchanged_at a2 sa2 sb1) /\
-                 (unchanged_except a1 sa2 sb2) in
-  let rec aux1 a :
+        (unchanged_at_extended (a1 `L.append` a2) sb1 sb2))) =
+  let aux a :
     Lemma
-      (requires (L.mem a a1 /\
-                 precond))
+      (requires (not !!(disjoint_access_location_from_locations a (a1 `L.append` a2))))
       (ensures (eval_access_location a sb1 == eval_access_location a sb2)) =
-    lemma_disjoint_access_location_from_locations_mem a1 a2 a;
-    assert (!!(disjoint_access_location_from_locations a a2));
-    assert (eval_access_location a sb1 == eval_access_location a sa1);
-    lemma_unchanged_at_mem a1 a sa1 sb2
+    lemma_disjoint_access_location_from_locations_append a a1 a2
   in
-  let rec aux2 a :
-    Lemma
-      (requires (L.mem a a2 /\
-                 precond))
-      (ensures (eval_access_location a sb1 == eval_access_location a sb2)) =
-    lemma_disjoint_access_locations_symmetric a1 a2 "";
-    lemma_disjoint_access_location_from_locations_mem a2 a1 a;
-    assert (!!(disjoint_access_location_from_locations a a1));
-    assert (eval_access_location a sb2 == eval_access_location a sa2);
-    lemma_unchanged_at_mem a2 a sa2 sb1
-  in
-  let rec aux a1' a1'' a2' a2'' :
-    Lemma
-      (requires (a1' `L.append` a1'' == a1 /\ a2' `L.append` a2'' == a2 /\
-                precond))
-      (ensures (unchanged_at (a1'' `L.append` a2'') sb1 sb2))
-      (decreases %[a1''; a2'']) =
-    match a1'' with
-    | [] -> (
-        match a2'' with
-        | [] -> ()
-        | y :: ys -> (
-            L.append_l_cons y ys a2';
-            L.append_mem a2' a2'' y;
-            aux2 y;
-            aux a1' a1'' (a2' `L.append` [y]) ys
-          )
-      )
-    | x :: xs ->
-      L.append_l_cons x xs a1';
-      L.append_mem a1' a1'' x;
-      aux1 x;
-      aux (a1' `L.append` [x]) xs a2' a2'' in
-  aux [] a1 [] a2
+  FStar.Classical.forall_intro (FStar.Classical.move_requires aux)
 
 let lemma_unchanged_except_same_transitive (as:list access_location) (s1 s2 s3:machine_state) :
   Lemma
@@ -1150,81 +1134,13 @@ let lemma_unchanged_except_same_transitive (as:list access_location) (s1 s2 s3:m
     (ensures (
         (unchanged_except as s1 s3))) = ()
 
-let lemma_unchanged_at_and_except_aux (a x:access_location) (xs:list access_location) (s1 s2:machine_state) :
+let rec lemma_unchanged_at_extended_and_except (as:list access_location) (s1 s2:machine_state) :
   Lemma
     (requires (
-        (unchanged_at (x :: xs) s1 s2) /\
-        (unchanged_except (x :: xs) s1 s2) /\
-        (!!(disjoint_access_location_from_locations a xs)) /\
-        (not !!(disjoint_access_location a x))))
-    (ensures (
-        (eval_access_location a s1 == eval_access_location a s2))) =
-  match a with
-  | ALoc64 oa -> (
-      match oa with
-      | OConst _ -> ()
-      | OReg ra -> (
-          match x with
-          | ALoc64 ox -> (
-              match ox with
-              | OConst _ -> ()
-              | OReg rx -> ()
-              | OMem mx ->
-                admit ()
-              | OStack mx ->
-                admit ()
-            )
-          | ALoc128 ox -> (
-              match ox with
-              | OReg128 rx ->
-                admit () (* WAT! *)
-              | _ ->
-                admit ()
-            )
-          | ALocCf | ALocOf -> ()
-        )
-      | OMem ma ->
-        admit ()
-      | OStack ma ->
-        admit ()
-    )
-  | ALoc128 oa -> (
-      match oa with
-      | OReg128 ra ->
-        admit ()
-      | OMem128 ma ->
-        admit ()
-      | OStack128 ma ->
-        admit ()
-    )
-  | ALocCf | ALocOf -> ()
-
-let rec lemma_unchanged_at_and_except (as:list access_location) (s1 s2:machine_state) :
-  Lemma
-    (requires (
-        (unchanged_at as s1 s2) /\
+        (unchanged_at_extended as s1 s2) /\
         (unchanged_except as s1 s2)))
     (ensures (
-        (unchanged_except [] s1 s2))) =
-  match as with
-  | [] -> ()
-  | x :: xs ->
-    FStar.Classical.forall_intro ((fun a -> (
-          FStar.Classical.arrow_to_impl
-          #(!!(disjoint_access_location_from_locations a xs))
-          #(eval_access_location a s1 == eval_access_location a s2))
-          (fun _ ->
-             FStar.Classical.or_elim
-             #_ #_ #(fun () -> eval_access_location a s1 == eval_access_location a s2)
-               (fun (_:unit{!!(disjoint_access_location a x)}) -> ())
-               (fun (_:unit{not !!(disjoint_access_location a x)}) ->
-                  lemma_unchanged_at_and_except_aux a x xs s1 s2)
-          )
-      ) <: (a:_) -> Lemma (
-        (!!(disjoint_access_location_from_locations a xs) ==>
-         (eval_access_location a s1 == eval_access_location a s2))
-      ));
-    lemma_unchanged_at_and_except xs s1 s2
+        (unchanged_except [] s1 s2))) = ()
 
 let lemma_equiv_states_when_except_none (s1 s2:machine_state) (ok:bool) :
   Lemma
@@ -1316,8 +1232,8 @@ let lemma_commute (f1 f2:st unit) (r1 w1 r2 w2:list access_location) (s:machine_
         !!(disjoint_access_locations l1 l2 ""))));
   lemma_disjoint_implies_unchanged_at r1 w2 s is2;
   lemma_disjoint_implies_unchanged_at r2 w1 s is1;
-  assert (unchanged_at w1 is1 is21);
-  assert (unchanged_at w2 is2 is12);
+  assert (unchanged_at_extended w1 is1 is21);
+  assert (unchanged_at_extended w2 is2 is12);
   assert (unchanged_except w2 s is2);
   assert (unchanged_except w1 s is1);
   assert (unchanged_except w2 is1 is12);
@@ -1329,8 +1245,9 @@ let lemma_commute (f1 f2:st unit) (r1 w1 r2 w2:list access_location) (s:machine_
   lemma_unchanged_except_append_symmetric w1 w2 s is12;
   lemma_unchanged_except_append_symmetric w2 w1 s is21;
   lemma_unchanged_except_same_transitive (w1 `L.append` w2) s is12 is21;
+  assume (unchanged_upon_both_non_disjoint w1 w2 is1 is2);
   lemma_unchanged_at_combine w1 w2 is1 is2 is12 is21;
-  lemma_unchanged_at_and_except (w1 `L.append` w2) is12 is21;
+  lemma_unchanged_at_extended_and_except (w1 `L.append` w2) is12 is21;
   assert (unchanged_except [] is12 is21);
   assert (s21.ms_ok = s12.ms_ok);
   assert (is12.ms_stack.initial_rsp = is21.ms_stack.initial_rsp);
@@ -1469,7 +1386,7 @@ let lemma_untainted_eval_ins_unchanged_behavior (i:ins{Instr? i}) (s1 s2:machine
     (ensures (
         let r, w = rw_set_of_ins i in
         let f = untainted_eval_ins i in
-        (unchanged_at w (run f s1) (run f s2)) /\
+        (unchanged_at_extended w (run f s1) (run f s2)) /\
         (run f s1).ms_ok = (run f s2).ms_ok)) =
   admit ()
 
